rupicola/io/Compilation.fsti
@@ -10,8 +10,11 @@ open LogRelTargetSource
 
 val compile #g #a (#s:fs_oval g a) (qs:g ⊢ s) : exp
 
-val lem_compile_equiv #g (#a:qType) (#s:fs_oval g a) (qs:g ⊢ s)
-  : Lemma (ensures (s ⊐ (compile qs))) (decreases qs)
+val lem_compile_superset #g (#a:qType) (#s:fs_oval g a) (qs:g ⊢ s)
+  : Lemma (ensures s ⊐ compile qs) (decreases qs)
+
+val lem_compile_subset #g (#a:qType) (#s:fs_oval g a) (qs:g ⊢ s)
+  : Lemma (ensures s ⊏ compile qs) (decreases qs)
 
 val lem_compile_closed_arrow_is_elam (#a #b:qType) (#s:fs_val (a ^->!@ b)) (qs: (a ^->!@ b) ⊩ s)
   : Lemma (ELam? (compile qs))
